fixed more proofs

src/LambdaTotalTriple_credits_perm.v
@@ -11,23 +11,27 @@ Require Import src.Permutation.
 Definition step_hoare_triple {V : Set}
   (e : Expr V) (P Q : StateAssertion V) : Prop :=
   forall (c : nat) ((*m*) m' : Map V),
+    Is_Valid_Map m' ->
     P (1+c) m' ->
     (*Permutation m m' ->*)
     exists (e' : Expr V) (m'' (*m'''*) : Map V),
       R[e, m' ~~> e', m''] /\
       (*Permutation m'' m''' /\*)
+      Is_Valid_Map m'' /\
       Q c m''.
 
 Definition hoare_triple {V : Set}
   (e : Expr V)
   (P : StateAssertion V) (Q : Value V -> StateAssertion V) : Prop :=
   forall (c1 : nat) ((*mp*) m : Map V),
+    Is_Valid_Map m ->
     P c1 m ->
     (*Permutation mp m ->*)
     exists (v : Value V) (c c2 : nat) (m' (*mq*) : Map V),
       C[e, m ~~> v, m' | c] /\
       Q v c2 m' /\
       (*Permutation m' mq /\*)
+      Is_Valid_Map m' /\
       c1 = c + c2.
 
 Definition triple {V : Set}
